finished constant folding pass

ConstFold.v
@@ -1,85 +1,88 @@
-From Coq Require Import String ZArith.
-From Vyper Require Import Config L10.Base L20.AST L20.Callset.
+From Coq Require Import String ZArith Lia.
+From Coq Require PropExtensionality.
+From Vyper Require Import Config UInt256 Calldag.
+From Vyper.L20 Require Import AST Callset Descend Expr Stmt.
 
 (** Do constant folding in expressions.
-   (We don't have const declarations yet, so this is going to be somewhat more complicated.) *)
+   (We don't have const declarations yet,
+    once we do, thise will be somewhat more complicated.) *)
 Fixpoint const_fold_expr {C: VyperConfig} (e: expr)
-: expr_result expr
+: string + expr
 := let fix const_fold_expr_list (l: list expr)
        := match l with
-          | nil => ExprSuccess nil
+          | nil => inr nil
           | (h :: t)%list =>
               match const_fold_expr h, const_fold_expr_list t with
-              | ExprAbort ab, _ | _, ExprAbort ab => ExprAbort ab 
-              | ExprSuccess h', ExprSuccess t' => ExprSuccess (h' :: t')%list
+              | inl err, _ | _, inl err => inl err
+              | inr h', inr t' => inr (h' :: t')%list
               end
           end
    in match e with
-   | Const _ | LocalVar _ | StorageVar _ => ExprSuccess e
+   | Const _ | LocalVar _ | StorageVar _ => inr e
    | UnOp op a =>
       let a' := const_fold_expr a in
       match a' with
-      | ExprAbort ab => a'
-      | ExprSuccess (Const x) =>
-          match L10.Base.interpret_unop op x with
-          | ExprAbort ab => ExprAbort ab
-          | ExprSuccess val => ExprSuccess (Const val)
+      | inl _ => a'
+      | inr (Const x) =>
+          match interpret_unop op x with
+          | Some val => inr (Const val)
+          | None => inl ("arithmetic error in unary " ++ L10.AST.string_of_unop op)%string
           end
-      | ExprSuccess x => ExprSuccess (UnOp op x)
+      | inr x => inr (UnOp op x)
       end
    | BinOp op a b =>
       let a' := const_fold_expr a in
       let b' := const_fold_expr b in
       match a', b' with
-      | ExprAbort ab, _ | _, ExprAbort ab => ExprAbort ab
-      | ExprSuccess (Const x), ExprSuccess (Const y) =>
-          match L10.Base.interpret_binop op x y with
-          | ExprAbort ab => ExprAbort ab
-          | ExprSuccess val => ExprSuccess (Const val)
+      | inl err, _ | _, inl err => inl err
+      | inr (Const x), inr (Const y) =>
+          match interpret_binop op x y with
+          | Some val => inr (Const val)
+          | None => inl ("arithmetic error in binary" ++ L10.AST.string_of_binop op)%string
           end
-      | ExprSuccess x, ExprSuccess y => ExprSuccess (BinOp op x y)
+      | inr x, inr y => inr (BinOp op x y)
       end
    | IfThenElse cond yes no =>
       let yes'  := const_fold_expr yes  in
       let no'   := const_fold_expr no   in
       match const_fold_expr cond with
-      | ExprAbort ab => ExprAbort ab
-      | ExprSuccess (Const x) => if (Z_of_uint256 x =? 0)%Z then no' else yes'
-      | ExprSuccess cond' =>
+      | inl err => inl err
+      | inr (Const x) => if (Z_of_uint256 x =? 0)%Z then no' else yes'
+      | inr cond' =>
           match yes', no' with
-          | ExprAbort ab, _ | _, ExprAbort ab => ExprAbort ab
-          | ExprSuccess x, ExprSuccess y => ExprSuccess (IfThenElse cond' x y)
+          | inl err, _ | _, inl err => inl err
+          | inr x, inr y => inr (IfThenElse cond' x y)
           end
       end
    | LogicalAnd a b =>
       match const_fold_expr a with
-      | ExprAbort ab => ExprAbort ab
-      | ExprSuccess (Const x) => if (Z_of_uint256 x =? 0)%Z
-                                   then ExprSuccess (Const x)
+      | inl err => inl err
+      | inr (Const x) => if (Z_of_uint256 x =? 0)%Z
+                                   then inr (Const x)
                                    else const_fold_expr b
-      | ExprSuccess a' => match const_fold_expr b with
-                          | ExprAbort ab => ExprAbort ab
-                          | ExprSuccess b' => ExprSuccess (LogicalAnd a' b')
-                          end
+      | inr a' => match const_fold_expr b with
+                  | inl err => inl err
+                  | inr b' => inr (LogicalAnd a' b')
+                  end
       end
    | LogicalOr a b =>
       match const_fold_expr a with
-      | ExprAbort ab => ExprAbort ab
-      | ExprSuccess (Const x) => if (Z_of_uint256 x =? 0)%Z
-                                   then const_fold_expr b
-                                   else ExprSuccess (Const x)
-      | ExprSuccess a' => match const_fold_expr b with
-                          | ExprAbort ab => ExprAbort ab
-                          | ExprSuccess b' => ExprSuccess (LogicalOr a' b')
-                          end
+      | inl err => inl err
+      | inr (Const x) => if (Z_of_uint256 x =? 0)%Z
+                           then const_fold_expr b
+                           else inr (Const x)
+      | inr a' => match const_fold_expr b with
+                  | inl err => inl err
+                  | inr b' => inr (LogicalOr a' b')
+                  end
       end
    | PrivateCall name args => match const_fold_expr_list args with
-                              | ExprAbort ab => ExprAbort ab
-                              | ExprSuccess args' => ExprSuccess (PrivateCall name args')
+                              | inl err => inl err
+                              | inr args' => inr (PrivateCall name args')
                               end
    | BuiltinCall name args => match const_fold_expr_list args with
-                              | ExprAbort ab => ExprAbort ab
-                              | ExprSuccess args' => ExprSuccess (BuiltinCall name args')
+                              | inl err => inl err
+                              | inr args' => inr (BuiltinCall name args')
                               end
    end.
 
@@ -87,7 +90,7 @@ Fixpoint const_fold_expr {C: VyperConfig} (e: expr)
 (** Constant folding cannot add new calls. *)
 Lemma callset_const_fold_expr {C: VyperConfig}
                               {e e': expr}
-                              (ok: const_fold_expr e = ExprSuccess e'):
+                              (ok: const_fold_expr e = inr e'):
   let _ := string_set_impl in
   FSet.is_subset (expr_callset e') (expr_callset e) = true.
 Proof.
@@ -104,23 +107,23 @@ cbn. revert e' ok. induction e using expr_ind'; intros; inversion ok; subst; cbn
 { (* LocalVar *) assumption. }
 { (* StorageVar *) assumption. }
 { (* UnOp *)
-  destruct (const_fold_expr e). 2:discriminate.
-  apply (IHe value eq_refl).
-  destruct value; cbn; inversion ok; try subst e'; try apply H.
+  destruct (const_fold_expr e). { discriminate. }
+  apply (IHe _ eq_refl).
+  destruct e0; cbn; inversion ok; try subst e'; try apply H. (* XXX: e0 *)
   destruct (interpret_unop op val). 2:discriminate.
-  inversion ok. subst e'. apply H.
+  { inversion ok. subst e'. apply H. }
 }
 { (* BinOp *)
   rewrite FSet.union_ok; apply Bool.orb_true_intro.
   assert (D: forall A A' B B': Prop, (A -> A') -> (B -> B') -> (A \/ B) -> (A' \/ B')) by tauto.
-  destruct (const_fold_expr e1). 2:discriminate.
-  destruct value; cbn.
+  destruct (const_fold_expr e1). discriminate.
+  destruct e; cbn.
   { (* e1 is Const *)
-    destruct (const_fold_expr e2). 2:discriminate.
+    destruct (const_fold_expr e2). discriminate.
     enough (E2: let _ := string_set_impl in FSet.has ((expr_callset e2)) s = true).
     { cbn in E2. rewrite E2. now right. }
-    cbn. apply (IHe2 value eq_refl).
-    destruct value; cbn; inversion ok; try subst e'; cbn in H;
+    cbn. apply (IHe2 _ eq_refl).
+    destruct e; cbn; inversion ok; try subst e'; cbn in H;
       try rewrite FSet.union_ok in H;
       try rewrite FSet.empty_ok in H;
       try rewrite Bool.orb_false_l in H;
@@ -143,19 +146,19 @@ cbn. revert e' ok. induction e using expr_ind'; intros; inversion ok; subst; cbn
   repeat rewrite FSet.union_ok. repeat rewrite Bool.orb_true_iff.
   assert (D: forall A A' B B' C C': Prop, (A -> A') -> (B -> B') -> (C -> C')
                                             -> (A \/ B \/ C) -> (A' \/ B' \/ C')) by tauto.
-  destruct (const_fold_expr e1). 2:discriminate.
-  destruct value.
+  destruct (const_fold_expr e1). discriminate.
+  destruct e.
   { (* Const *)
     destruct (Z_of_uint256 val =? 0)%Z.
     {
-      destruct (const_fold_expr e3). 2:discriminate.
+      destruct (const_fold_expr e3). discriminate.
       inversion ok. subst e'.
       repeat rewrite FSet.union_ok.
       rewrite (IHe3 _ eq_refl H).
       right. right. trivial.
     }
     (* same as in the previous branch but we dig into "yes" (e2) this time *)
-    destruct (const_fold_expr e2). 2:discriminate.
+    destruct (const_fold_expr e2). discriminate.
     inversion ok. subst e'.
     repeat rewrite FSet.union_ok.
     rewrite (IHe2 _ eq_refl H).
@@ -173,8 +176,8 @@ cbn. revert e' ok. induction e using expr_ind'; intros; inversion ok; subst; cbn
 { (* LogicalAnd *)
   rewrite FSet.union_ok; apply Bool.orb_true_intro.
   assert (D: forall A A' B B': Prop, (A -> A') -> (B -> B') -> (A \/ B) -> (A' \/ B')) by tauto.
-  destruct (const_fold_expr e1). 2:discriminate.
-  destruct value; cbn.
+  destruct (const_fold_expr e1). discriminate.
+  destruct e; cbn.
   { (* e1 is Const *)
     destruct (Z_of_uint256 val =? 0)%Z.
     { inversion ok. subst e'. cbn in H. rewrite FSet.empty_ok in H. discriminate. }
@@ -191,8 +194,8 @@ cbn. revert e' ok. induction e using expr_ind'; intros; inversion ok; subst; cbn
 { (* LogicalOr *)
   rewrite FSet.union_ok; apply Bool.orb_true_intro.
   assert (D: forall A A' B B': Prop, (A -> A') -> (B -> B') -> (A \/ B) -> (A' \/ B')) by tauto.
-  destruct (const_fold_expr e1). 2:discriminate.
-  destruct value; cbn.
+  destruct (const_fold_expr e1). discriminate.
+  destruct e; cbn.
   { (* e1 is Const *)
     destruct (Z_of_uint256 val =? 0)%Z.
     right. apply (IHe2 _ ok H).
@@ -216,10 +219,10 @@ cbn. revert e' ok. induction e using expr_ind'; intros; inversion ok; subst; cbn
     destruct (string_dec name s). { contradiction. } exact H.
   }
   assert (FH := List.Forall_inv F). cbn in FH.
-  destruct (const_fold_expr head). 2:discriminate.
-  assert (FHvalue := FH value eq_refl). clear FH.
+  destruct (const_fold_expr head). discriminate.
+  assert (FHvalue := FH _ eq_refl). clear FH.
   rewrite FSet.union_ok.
-  destruct (_ args). 2:discriminate.
+  destruct (_ args). discriminate.
   inversion ok. subst e'.
   cbn in H. rewrite FSet.add_ok in H.
   destruct (string_dec name s) as [|_]. { contradiction. }
@@ -236,10 +239,10 @@ clear H2. rename H into F. rename H0 into H. (* XXX *)
 revert e' ok H. induction args as [|head]; intros.
 { inversion ok. subst e'. cbn in H. exact H. }
 assert (FH := List.Forall_inv F). cbn in FH.
-destruct (const_fold_expr head). 2:discriminate.
-assert (FHvalue := FH value eq_refl). clear FH.
+destruct (const_fold_expr head). discriminate.
+assert (FHvalue := FH _ eq_refl). clear FH.
 rewrite FSet.union_ok.
-destruct (_ args). 2:discriminate.
+destruct (_ args). discriminate.
 inversion ok. subst e'.
 cbn in H.
 rewrite FSet.union_ok in H.
@@ -251,30 +254,30 @@ tauto.
 Qed.
 
 
-Definition expr_result_map {C: VyperConfig} {A B} (f: A -> B) (e: expr_result A)
-: expr_result B
+Definition sum_map {C: VyperConfig} {Err A B} (f: A -> B) (e: Err + A)
+: Err +  B
 := match e with
-   | ExprSuccess a => ExprSuccess (f a)
-   | ExprAbort ab => ExprAbort ab
+   | inl err => inl err
+   | inr a => inr (f a)
    end.
 
 Definition const_fold_small_stmt {C: VyperConfig} (ss: small_stmt)
-: expr_result small_stmt
+: string + small_stmt
 := match ss with
-   | Pass | Abort _ => ExprSuccess ss
-   | Return     e => expr_result_map Return       (const_fold_expr e)
-   | Raise      e => expr_result_map Raise        (const_fold_expr e)
-   | Assign lhs e => expr_result_map (Assign lhs) (const_fold_expr e)
-   | ExprStmt   e => expr_result_map ExprStmt     (const_fold_expr e)
+   | Pass | Abort _ => inr ss
+   | Return     e => sum_map Return       (const_fold_expr e)
+   | Raise      e => sum_map Raise        (const_fold_expr e)
+   | Assign lhs e => sum_map (Assign lhs) (const_fold_expr e)
+   | ExprStmt   e => sum_map ExprStmt     (const_fold_expr e)
    end.
 
 Lemma callset_const_fold_small_stmt {C: VyperConfig}
                                     {ss ss': small_stmt}
-                                    (ok: const_fold_small_stmt ss = ExprSuccess ss'):
+                                    (ok: const_fold_small_stmt ss = inr ss'):
   let _ := string_set_impl in
   FSet.is_subset (small_stmt_callset ss') (small_stmt_callset ss) = true.
 Proof.
-cbn. destruct ss; cbn in ok; unfold expr_result_map in *.
+cbn. destruct ss; cbn in ok; unfold sum_map in *.
 1-2: (* Pass, Abort *) inversion ok; subst ss'; apply FSet.is_subset_refl.
 1-4:
   remember (const_fold_expr _) as z; symmetry in Heqz; destruct z; try discriminate;
@@ -283,47 +286,45 @@ cbn. destruct ss; cbn in ok; unfold expr_result_map in *.
 Qed.
 
 
-Definition expr_result_ap {C: VyperConfig} {A B} (f: expr_result (A -> B)) (e: expr_result A)
-: expr_result B
+Definition sum_ap {C: VyperConfig} {Err A B} (f: Err + (A -> B)) (e: Err + A)
+: Err + B
 := match f with
-   | ExprSuccess g => match e with
-                      | ExprSuccess a => ExprSuccess (g a)
-                      | ExprAbort ab => ExprAbort ab
-                      end
-   | ExprAbort ab => ExprAbort ab
+   | inr g => match e with
+              | inr a => inr (g a)
+              | inl err => inl err
+              end
+   | inl err => inl err
    end.
 
 Fixpoint const_fold_stmt {C: VyperConfig} (s: stmt)
-: expr_result stmt
+: string + stmt
 := match s with
-   | SmallStmt ss => expr_result_map SmallStmt (const_fold_small_stmt ss)
+   | SmallStmt ss => sum_map SmallStmt (const_fold_small_stmt ss)
    | LocalVarDecl name init body =>
-        expr_result_ap (expr_result_map (LocalVarDecl name) (const_fold_expr init))
-                       (const_fold_stmt body)
+        sum_ap (sum_map (LocalVarDecl name) (const_fold_expr init))
+               (const_fold_stmt body)
    | IfElseStmt cond yes no =>
         (* no attempt is made here to throw away the unused branch if [cond] is a constant. *)
-        expr_result_ap (expr_result_ap (expr_result_map IfElseStmt (const_fold_expr cond))
-                                       (const_fold_stmt yes))
-                       (const_fold_stmt no)
+        sum_ap (sum_ap (sum_map IfElseStmt (const_fold_expr cond))
+                       (const_fold_stmt yes))
+               (const_fold_stmt no)
    | Loop name init count body =>
-        expr_result_ap (expr_result_map
-                         (fun f => f count)
-                         (expr_result_map (Loop name) (const_fold_expr init)))
-                       (const_fold_stmt body)
+        sum_ap (sum_map (fun f => f count)
+                        (sum_map (Loop name) (const_fold_expr init)))
+               (const_fold_stmt body)
    | Semicolon a b =>
-        expr_result_ap (expr_result_map Semicolon (const_fold_stmt a))
-                       (const_fold_stmt b)
+        sum_ap (sum_map Semicolon (const_fold_stmt a)) (const_fold_stmt b)
    end.
 
 Lemma callset_const_fold_stmt {C: VyperConfig}
                               {s s': stmt}
-                              (ok: const_fold_stmt s = ExprSuccess s'):
+                              (ok: const_fold_stmt s = inr s'):
   let _ := string_set_impl in
   FSet.is_subset (stmt_callset s') (stmt_callset s) = true.
 Proof.
 cbn.
 revert s' ok.
-induction s; intros; cbn in ok; unfold expr_result_map in *; unfold expr_result_ap in *; cbn.
+induction s; intros; cbn in ok; unfold sum_map in *; unfold sum_ap in *; cbn.
 { (* SmallStmt *)
   remember (const_fold_small_stmt _) as z; symmetry in Heqz; destruct z; try discriminate.
   inversion ok; subst s'.
@@ -372,47 +373,1429 @@ Qed.
 
 
 Definition const_fold_decl {C: VyperConfig} (d: decl)
-: expr_result decl
+: string + decl
 := match d with
-   | StorageVarDecl name => ExprSuccess d
+   | StorageVarDecl name => inr d
    | FunDecl name arg_names body =>
-       expr_result_map (FunDecl name arg_names) (const_fold_stmt body)
+       sum_map (FunDecl name arg_names) (const_fold_stmt body)
    end.
 
-(*
+Lemma callset_const_fold_decl {C: VyperConfig}
+                              {d d': decl}
+                              (ok: const_fold_decl d = inr d'):
+  let _ := string_set_impl in
+  FSet.is_subset (decl_callset d') (decl_callset d) = true.
+Proof.
+destruct d; cbn in *.
+{ inversion ok. subst d'. cbn. apply FSet.is_subset_refl. }
+remember (const_fold_stmt body) as body'. symmetry in Heqbody'. destruct body'. { easy. }
+cbn in ok. inversion ok. subst d'. cbn.
+now apply callset_const_fold_stmt.
+Qed.
+
+Local Lemma const_fold_calldag_depthmap_ok {C: VyperConfig}
+                                           (name: string)
+                                           (cd: calldag)
+                                           (d: string_map decl):
+   let _ := string_map_impl in
+   forall E: map_maybe_map (cd_decls cd) const_fold_decl = inr d,
+     match Map.lookup d name with
+     | Some decl =>
+         match cd_depthmap cd name with
+         | Some x =>
+             let _ := string_set_impl in
+             FSet.for_all (Callset.decl_callset decl)
+               (fun callee : string =>
+                match cd_depthmap cd callee with
+                | Some y => y <? x
+                | None => false
+                end) = true
+         | None => False
+         end
+     | None => True
+     end.
+Proof.
+intros.
+remember (Map.lookup d name) as m.
+destruct m. 2:trivial.
+assert (D := cd_depthmap_ok cd name).
+assert (F := map_maybe_map_ok E name).
+destruct (Map.lookup (cd_decls cd) name). 2:{ now rewrite F in Heqm. }
+destruct (cd_depthmap cd name). 2:assumption.
+rewrite FSet.for_all_ok. rewrite FSet.for_all_ok in D.
+intros x H.
+remember (const_fold_decl d1) as d30.
+destruct d30. { contradiction. }
+rewrite<- Heqm in F. inversion F; subst.
+assert (Q := callset_const_fold_decl (eq_sym Heqd30)).
+cbn in Q. rewrite FSet.is_subset_ok in Q.
+assert (Qx := Q x).
+rewrite H in Qx. cbn in Qx.
+apply (D x Qx).
+Qed.
+
+(* All this should be way simpler as it's practically identical to From20To30.FunCtx. *)
+Definition const_fold_calldag {C: VyperConfig} (cd: calldag)
+: string + calldag
+:= let _ := string_map_impl in
+   match map_maybe_map (cd_decls cd) const_fold_decl as cd' return _ = cd' -> _ with
+   | inl err => fun _ => inl err
+   | inr d => fun E => inr
+     {| cd_decls := d
+      ; cd_depthmap := cd_depthmap cd
+      ; cd_depthmap_ok name := const_fold_calldag_depthmap_ok name cd d E
+     |}
+   end eq_refl.
+
+
+(*************************************************************************************)
+(* fun ctx *)
+
+Section FunCtx1.
+  Context {C: VyperConfig}
+          {bound: nat}
+          {cd cd': calldag}
+          (ok: const_fold_calldag cd = inr cd').
+
+  Lemma const_fold_fun_ctx_depthmap (name: string):
+    cd_depthmap cd name
+     =
+    cd_depthmap cd' name.
+  Proof.
+  destruct cd.
+  unfold const_fold_calldag in ok.
+  cbn in *.
+  remember (fun d (E : map_maybe_map cd_decls const_fold_decl = inr d) =>
+         inr
+           {|
+           cd_decls := d;
+           cd_depthmap := cd_depthmap;
+           cd_depthmap_ok := fun name : string =>
+                             const_fold_calldag_depthmap_ok name
+                               {|
+                               cd_decls := cd_decls;
+                               cd_depthmap := cd_depthmap;
+                               cd_depthmap_ok := cd_depthmap_ok |} d E |}) as good_branch.
+  assert (K: forall (d': string_map decl)
+                    (E: map_maybe_map cd_decls const_fold_decl = inr d'),
+               good_branch d' E = inr cd'
+                ->
+               Calldag.cd_depthmap cd' name = cd_depthmap name).
+  {
+    intros. subst.
+    inversion H. now subst.
+  }
+  clear Heqgood_branch.
+  destruct (map_maybe_map cd_decls const_fold_decl) as [|d']. { discriminate. }
+  symmetry.
+  apply (K d' eq_refl ok).
+  Qed.
+
+  Lemma const_fold_fun_ctx_declmap (name: string):
+    match cd_declmap cd name with
+    | Some d => Some (const_fold_decl d)
+    | None => None
+    end
+     =
+    match cd_declmap cd' name with
+    | Some d => Some (inr d)
+    | None => None
+    end.
+  Proof.
+  destruct cd.
+  unfold const_fold_calldag in ok.
+  cbn in *.
+  remember (fun d (E : map_maybe_map cd_decls const_fold_decl = inr d) =>
+         inr
+           {|
+           cd_decls := d;
+           cd_depthmap := cd_depthmap;
+           cd_depthmap_ok := fun name : string =>
+                             const_fold_calldag_depthmap_ok name
+                               {|
+                               cd_decls := cd_decls;
+                               cd_depthmap := cd_depthmap;
+                               cd_depthmap_ok := cd_depthmap_ok |} d E |}) as good_branch.
+  unfold cd_declmap. cbn.
+  assert (K: forall (d': string_map decl)
+                    (E: map_maybe_map cd_decls const_fold_decl = inr d'),
+               good_branch d' E = inr cd'
+                ->
+               let _ := string_map_impl in
+               match Map.lookup cd_decls name with
+               | Some d => Some (const_fold_decl d)
+               | None => None
+               end = match Map.lookup (Calldag.cd_decls cd') name with
+                     | Some d => Some (inr d)
+                     | None => None
+                     end).
+  {
+    intros. subst.
+    inversion H. subst.
+    cbn.
+    clear H ok.
+    assert (M := map_maybe_map_ok E name).
+    destruct (Map.lookup cd_decls name). 2:{ now destruct Map.lookup. }
+    destruct (const_fold_decl d). { contradiction. }
+    (* why rewrite M doesn't work? *)
+    destruct Map.lookup. { now inversion M. }
+    discriminate.
+  }
+  clear Heqgood_branch.
+  destruct (map_maybe_map cd_decls const_fold_decl) as [|d']. { discriminate. }
+  apply (K d' eq_refl ok).
+  Qed.
+End FunCtx1.
+
+Section FunCtx2.
+  Context {C: VyperConfig}
+          {bound: nat}
+          {cd cd': calldag}
+          (ok: const_fold_calldag cd = inr cd')
+          (fc: fun_ctx cd bound).
+
+  Local Lemma translate_fun_ctx_fun_decl_helper:
+    cd_declmap cd' (fun_name fc) <> None.
+  Proof.
+  intro E.
+  assert (Ok := fun_decl_ok fc).
+  assert (M := const_fold_fun_ctx_declmap ok (fun_name fc)).
+  rewrite Ok in M.
+  rewrite E in M.
+  discriminate.
+  Qed.
+
+  Definition cached_const_folded_decl
+  := match cd_declmap cd' (fun_name fc)
+     as d' return _ = d' -> _
+     with
+     | Some f => fun _ => f
+     | None => fun E =>
+          False_rect _ (translate_fun_ctx_fun_decl_helper E)
+     end eq_refl.
+
+  Local Lemma const_fold_fun_ctx_decl_ok:
+    cd_declmap cd' (fun_name fc)
+     =
+    Some cached_const_folded_decl.
+  Proof.
+  assert (D := fun_decl_ok fc).
+  unfold cached_const_folded_decl.
+  remember translate_fun_ctx_fun_decl_helper as foo. clear Heqfoo. revert foo.
+  destruct (cd_declmap cd' (fun_name fc)). { trivial. }
+  intro. contradiction.
+  Qed.
+
+  Local Lemma const_fold_fun_ctx_depth_ok:
+    cd_depthmap cd' (fun_name fc) = Some (fun_depth fc).
+  Proof.
+  rewrite<- (const_fold_fun_ctx_depthmap ok).
+  apply (fun_depth_ok fc).
+  Qed.
+
+  Definition const_fold_fun_ctx
+  : fun_ctx cd' bound
+  := {| fun_name := fun_name fc
+      ; fun_depth := fun_depth fc
+      ; fun_depth_ok := const_fold_fun_ctx_depth_ok
+      ; fun_decl := cached_const_folded_decl
+      ; fun_decl_ok := const_fold_fun_ctx_decl_ok
+      ; fun_bound_ok := fun_bound_ok fc
+     |}.
+End FunCtx2.
+
+(*************************************************************************************)
+
+Lemma weak_interpret_const_fold_expr_list
+              {C: VyperConfig}
+              {(*bigger_call_depth_bound*) smaller_call_depth_bound: nat}
+              (*(Ebound: bigger_call_depth_bound = S smaller_call_depth_bound)*)
+              (builtins: string -> option L10.Base.builtin)
+              {cd cd': calldag}
+              (ok: const_fold_calldag cd = inr cd')
+              (fc: fun_ctx cd (S smaller_call_depth_bound))
+              {do_call: forall
+                    (smaller_fc: fun_ctx cd smaller_call_depth_bound)
+                    (world: world_state)
+                    (arg_values: list uint256),
+                  world_state * L10.Base.expr_result uint256}
+              {do_call': forall
+                    (smaller_fc: fun_ctx cd' smaller_call_depth_bound)
+                    (world: world_state)
+                    (arg_values: list uint256),
+                  world_state * L10.Base.expr_result uint256}
+              (DoCallOk: forall smaller_fc world arg_values,
+                           do_call' (const_fold_fun_ctx ok smaller_fc) world arg_values
+                            =
+                           do_call smaller_fc world arg_values)
+              (world: world_state)
+              (loc: string_map uint256)
+              {l l': list expr}
+              (ExprOk: (fix const_fold_expr_list (l: list expr)
+                        := match l with
+                           | nil => inr nil
+                           | (h :: t)%list =>
+                               match const_fold_expr h, const_fold_expr_list t with
+                               | inl err, _ | _, inl err => inl err
+                               | inr h', inr t' => inr (h' :: t')%list
+                               end
+                           end) l = inr l')
+              (CallOk': let _ := string_set_impl in
+                 FSet.is_subset (expr_list_callset l')
+                                (decl_callset
+                                   (fun_decl
+                                     (const_fold_fun_ctx ok fc)))
+                 = true)
+              (CallOk: let _ := string_set_impl in
+                 FSet.is_subset (expr_list_callset l)
+                                (decl_callset (fun_decl fc))
+                 = true)
+              (ItemsOk: List.Forall
+                  (fun e : expr =>
+                   forall e' : expr,
+                   const_fold_expr e = inr e' ->
+                   forall
+                     (CallOk : let H := string_set_impl in
+                               FSet.is_subset (expr_callset e) (decl_callset (fun_decl fc)) = true)
+                     (CallOk' : let H := string_set_impl in
+                                FSet.is_subset (expr_callset e')
+                                  (decl_callset (fun_decl (const_fold_fun_ctx ok fc))) = true)
+                     (world : world_state) (loc : string_map uint256),
+                   interpret_expr eq_refl (const_fold_fun_ctx ok fc) do_call' builtins world loc e' CallOk' =
+                   interpret_expr eq_refl fc do_call builtins world loc e CallOk) l):
+   interpret_expr_list eq_refl (const_fold_fun_ctx ok fc)
+                       do_call' builtins
+                       world loc l' CallOk'
+    =
+   interpret_expr_list eq_refl fc
+                       do_call builtins
+                       world loc l CallOk.
+Proof.
+revert l' ExprOk CallOk' world loc. induction l as [|lhead]; intros.
+{ inversion ExprOk. now subst l'. }
+remember (const_fold_expr lhead) as chead. symmetry in Heqchead.
+destruct chead. { discriminate. }
+assert (HeadItemOk := List.Forall_inv ItemsOk).
+assert (TailItemsOk := List.Forall_inv_tail ItemsOk).
+remember ((fix const_fold_expr_list (l : list expr) : string + list expr :=
+              match l with
+              | nil => inr nil
+              | (h :: t)%list =>
+                  match const_fold_expr h with
+                  | inl err => inl err
+                  | inr h' =>
+                      match const_fold_expr_list t with
+                      | inl err => inl err
+                      | inr t' => inr (h' :: t')%list
+                      end
+                  end
+              end) l) as c'.
+symmetry in Heqc'.
+destruct c'. { discriminate. }
+inversion ExprOk. subst l'.
+cbn.
+rewrite (HeadItemOk _ Heqchead
+                    (callset_descend_head eq_refl CallOk)
+                    (callset_descend_head eq_refl CallOk')).
+destruct interpret_expr as (world', result_h). destruct result_h. 2:{ trivial. }
+now rewrite (IHl (callset_descend_tail eq_refl CallOk) TailItemsOk _ eq_refl
+                 (callset_descend_tail eq_refl CallOk')).
+Qed.
+
+
 Lemma interpret_const_fold_expr {C: VyperConfig}
                                 {bigger_call_depth_bound smaller_call_depth_bound: nat}
                                 (Ebound: bigger_call_depth_bound = S smaller_call_depth_bound)
-                                (builtins: string -> option builtin)
-                                {cd cd': L20.Descend.calldag}
-                                (fc fc': fun_ctx cd bigger_call_depth_bound)
+                                (builtins: string -> option L10.Base.builtin)
+                                {cd cd': calldag}
+                                (ok: const_fold_calldag cd = inr cd')
+                                (fc: fun_ctx cd bigger_call_depth_bound)
                                 {do_call: forall
                                       (smaller_fc: fun_ctx cd smaller_call_depth_bound)
                                       (world: world_state)
                                       (arg_values: list uint256),
-                                    world_state * expr_result uint256}
+                                    world_state * L10.Base.expr_result uint256}
                                 {do_call': forall
                                       (smaller_fc: fun_ctx cd' smaller_call_depth_bound)
                                       (world: world_state)
                                       (arg_values: list uint256),
-                                    world_state * expr_result uint256}
+                                    world_state * L10.Base.expr_result uint256}
                                 (DoCallOk: forall smaller_fc world arg_values,
-                                             do_call smaller_fc world arg_values
+                                             do_call' (const_fold_fun_ctx ok smaller_fc) world arg_values
                                               =
-                                             do_call' smaller_fc' world arg_values)
+                                             do_call smaller_fc world arg_values)
                                 (world: world_state)
                                 (loc: string_map uint256)
                                 {e e': expr}
-                                (ExprOk: const_fold_expr e = ExprSuccess e')
+                                (ExprOk: const_fold_expr e = inr e')
+                                (CallOk': let _ := string_set_impl in
+                                   FSet.is_subset (expr_callset e')
+                                                  (decl_callset
+                                                     (fun_decl
+                                                       (const_fold_fun_ctx ok fc)))
+                                   = true)
                                 (CallOk: let _ := string_set_impl in
                                    FSet.is_subset (expr_callset e)
-                                                  (L20.Callset.decl_callset
-                                                     (fun_decl
-                                                       (translate_fun_ctx fc ok)))
-                                   = true)
-                                (CallOk10: let _ := string_set_impl in 
-                                   FSet.is_subset (L10.Callset.expr_callset e10)
-                                                  (L10.Callset.decl_callset
-                                                    (fun_decl fc))
+                                                  (decl_callset (fun_decl fc))
                                    = true):
- *)
+   interpret_expr Ebound (const_fold_fun_ctx ok fc)
+                  do_call' builtins
+                  world loc e' CallOk'
+    =
+   interpret_expr Ebound fc
+                  do_call builtins
+                  world loc e CallOk.
+Proof.
+revert e' ExprOk CallOk CallOk' world loc. induction e using expr_ind'; intros;
+  cbn in ExprOk; inversion ExprOk; subst.
+(* Const, LocalVar *) 1-2: reflexivity.
+{ (* StorageVar *)
+  cbn.
+  unfold storage_var_is_declared.
+  assert (F := const_fold_fun_ctx_declmap ok name).
+  destruct (cd_declmap cd name), (cd_declmap cd' name); try easy.
+  destruct d; cbn in F; inversion F. { now subst. }
+  remember (const_fold_stmt body) as body'.
+  destruct body'. { discriminate. }
+  inversion F. now subst.
+}
+{ (* UnOp *)
+  remember (const_fold_expr e) as ce.
+  destruct ce as [|arg]. { discriminate. }
+  destruct arg.
+  { (* arg is const, so interpret immediately *)
+    remember (interpret_unop op val) as unop_result. destruct unop_result. 2:discriminate.
+    inversion ExprOk. subst e'. cbn.
+    rewrite<- (IHe _ eq_refl _ CallOk').
+    cbn. unfold Base.interpret_unop.
+    now rewrite<- Hequnop_result.
+  }
+  (* arg is not const *)
+  1-9: inversion ExprOk; subst e';
+       assert (IH := IHe _ eq_refl
+                      (callset_descend_unop eq_refl CallOk) 
+                      (callset_descend_unop eq_refl CallOk')
+                      world loc);
+       cbn; now rewrite<- IH.
+}
+{ (* BinOp *)
+  assert (BinOpOk:
+    forall (e1' e2': expr) CallOk' CallOk
+           (Left: interpret_expr eq_refl (const_fold_fun_ctx ok fc) do_call' builtins world loc
+                                e1' (callset_descend_binop_left eq_refl CallOk') 
+                    =
+                  interpret_expr eq_refl fc do_call builtins world loc e1
+                                 (callset_descend_binop_left eq_refl CallOk))
+           (Right: forall world loc,
+                     interpret_expr eq_refl (const_fold_fun_ctx ok fc) do_call' builtins world loc e2'
+                                    (callset_descend_binop_right eq_refl CallOk') 
+                      =
+                     interpret_expr eq_refl fc do_call builtins world loc e2
+                                    (callset_descend_binop_right eq_refl CallOk)),
+          interpret_expr eq_refl (const_fold_fun_ctx ok fc) do_call' builtins world loc
+                         (BinOp op e1' e2') CallOk'
+           =
+          interpret_expr eq_refl fc do_call builtins world loc (BinOp op e1 e2) CallOk).
+  {
+    intros.
+    cbn. rewrite<- Left. cbn.
+    (* This doesn't work with the normal term.
+       Perhaps this is related to the reason BinOpOk is needed at all.
+     *)
+    destruct (@interpret_expr C (S smaller_call_depth_bound) smaller_call_depth_bound
+               (@eq_refl nat (S smaller_call_depth_bound)) cd'
+               (@const_fold_fun_ctx C (S smaller_call_depth_bound) cd cd' ok fc) do_call' builtins world loc e1'
+               (@callset_descend_binop_left C (@BinOp C op e1' e2') e1' e2' op
+                  (@decl_callset C (@cached_const_folded_decl C (S smaller_call_depth_bound) cd cd' ok fc))
+                  (@eq_refl (@expr C) (@BinOp C op e1' e2')) CallOk'0)) as (world', result_a).
+    destruct result_a. 2:reflexivity.
+    cbn. now rewrite Right.
+  }
+  remember (const_fold_expr e1) as ce1.
+  destruct ce1 as [|arg1]. { discriminate. }
+  destruct arg1; remember (const_fold_expr e2) as ce2; destruct ce2 as [|arg2]; try discriminate.
+  { (* arg1 is const, so check out arg2 *)
+    destruct arg2.
+    { (* arg2 is const, so interpret immediately *)
+      remember (interpret_binop op _ _) as binop_result. destruct binop_result. 2:discriminate.
+      inversion ExprOk. subst e'. cbn.
+      rewrite<- (IHe1 _ eq_refl _ CallOk').
+      cbn.
+      rewrite<- (IHe2 _ eq_refl _ CallOk').
+      unfold Base.interpret_binop. cbn.
+      now rewrite<- Heqbinop_result.
+    }
+    (* arg2 is not const *)
+    1-9: inversion ExprOk; subst e';
+         assert (IH1 := IHe1 _ eq_refl
+                        (callset_descend_binop_left eq_refl CallOk)
+                        (callset_descend_binop_left eq_refl CallOk')
+                        world loc);
+         assert (IH2 := IHe2 _ eq_refl
+                        (callset_descend_binop_right eq_refl CallOk)
+                        (callset_descend_binop_right eq_refl CallOk')
+                        world loc);
+         cbn; rewrite<- IH1; cbn; now rewrite<- IH2.
+  }
+  (* arg1 is not const *)
+  1-9: inversion ExprOk; subst e';
+        assert (IH1 := IHe1 _ eq_refl
+                       (callset_descend_binop_left eq_refl CallOk)
+                       (callset_descend_binop_left eq_refl CallOk')
+                       world loc);
+        assert (IH2 := IHe2 _ eq_refl
+                       (callset_descend_binop_right eq_refl CallOk)
+                       (callset_descend_binop_right eq_refl CallOk'));
+        apply (BinOpOk _ _ CallOk' CallOk IH1 IH2).
+}
+{ (* IfThenElse *)
+  rename e1 into cond. rename IHe1 into IHcond.
+  rename e2 into yes. rename IHe2 into IHyes.
+  rename e3 into no. rename IHe3 into IHno.
+  remember (const_fold_expr cond) as cc. destruct cc as [|cc]. { discriminate. }
+  cbn.
+  destruct cc.
+  { (* cond is a const *)
+    rewrite<- (IHcond _ eq_refl
+                      (callset_descend_if_cond eq_refl CallOk)
+                      FSet.empty_subset).
+    cbn.
+    destruct (Z_of_uint256 val =? 0)%Z.
+    { now apply IHno. }
+    now apply IHyes.
+  }
+  (* cond is not const *)
+  1-9: remember (const_fold_expr yes) as cyes; destruct cyes as [|cyes]; try discriminate;
+       remember (const_fold_expr no)  as cno;  destruct cno  as [|cno];  try discriminate;
+       inversion ExprOk; subst e';
+       try match goal with
+           | H: inr ?c = const_fold_expr _ |- _ => remember c as cond'
+           end;
+       rewrite<- (IHcond _ eq_refl
+                        (callset_descend_if_cond eq_refl CallOk)
+                        (callset_descend_if_cond eq_refl CallOk'));
+       cbn;
+       destruct interpret_expr;
+       rewrite (IHyes _ eq_refl
+                      (callset_descend_if_then eq_refl CallOk)
+                      (callset_descend_if_then eq_refl CallOk'));
+       rewrite (IHno _ eq_refl
+                     (callset_descend_if_else eq_refl CallOk)
+                     (callset_descend_if_else eq_refl CallOk'));
+       trivial.
+}
+{ (* LogicalAnd *)
+  remember (const_fold_expr e1) as c1. destruct c1 as [|c1]. { discriminate. }
+  cbn.
+  destruct c1.
+  { (* left arg is a const *)
+    rewrite<- (IHe1 _ eq_refl
+                    (callset_descend_and_left eq_refl CallOk)
+                    FSet.empty_subset).
+    cbn.
+    destruct (Z_of_uint256 val =? 0)%Z.
+    { inversion ExprOk. now subst e'. }
+    now apply IHe2.
+  }
+  (* left arg is not const *)
+  1-9: remember (const_fold_expr e2) as c2; destruct c2 as [|c2]; try discriminate;
+       inversion ExprOk; subst e';
+       try match goal with
+           | H: inr ?c = const_fold_expr _ |- _ => remember c as cond'
+           end;
+       rewrite<- (IHe1 _ eq_refl
+                      (callset_descend_and_left eq_refl CallOk)
+                      (callset_descend_and_left eq_refl CallOk'));
+       cbn;
+       destruct interpret_expr;
+       now rewrite (IHe2 _ eq_refl
+                         (callset_descend_and_right eq_refl CallOk)
+                         (callset_descend_and_right eq_refl CallOk')).
+}
+{ (* LogicalOr *)
+  remember (const_fold_expr e1) as c1. destruct c1 as [|c1]. { discriminate. }
+  cbn.
+  destruct c1.
+  { (* left arg is a const *)
+    rewrite<- (IHe1 _ eq_refl
+                    (callset_descend_or_left eq_refl CallOk)
+                    FSet.empty_subset).
+    cbn.
+    destruct (Z_of_uint256 val =? 0)%Z.
+    { now apply IHe2. }
+    inversion ExprOk. now subst e'.
+  }
+  (* left arg is not const *)
+  1-9: remember (const_fold_expr e2) as c2; destruct c2 as [|c2]; try discriminate;
+       inversion ExprOk; subst e';
+       try match goal with
+           | H: inr ?c = const_fold_expr _ |- _ => remember c as cond'
+           end;
+       rewrite<- (IHe1 _ eq_refl
+                      (callset_descend_or_left eq_refl CallOk)
+                      (callset_descend_or_left eq_refl CallOk'));
+       cbn;
+       destruct interpret_expr;
+       now rewrite (IHe2 _ eq_refl
+                         (callset_descend_or_right eq_refl CallOk)
+                         (callset_descend_or_right eq_refl CallOk')).
+}
+{ (* PrivateCall *)
+  remember ((fix const_fold_expr_list (l : list expr) : string + list expr :=
+              match l with
+              | nil => inr nil
+              | (h :: t)%list =>
+                  match const_fold_expr h with
+                  | inl err => inl err
+                  | inr h' =>
+                      match const_fold_expr_list t with
+                      | inl err => inl err
+                      | inr t' => inr (h' :: t')%list
+                      end
+                  end
+              end) args) as cargs. symmetry in Heqcargs. destruct cargs. { discriminate. }
+  inversion ExprOk. subst e'. cbn.
+  rename l into args'.
+  assert (R':
+    forall Ok' Ok,  (* initially: (callset_descend_args eq_refl CallOk') etc *)
+    interpret_expr_list eq_refl (const_fold_fun_ctx ok fc) do_call' builtins world loc args' Ok'
+     =
+    (fix
+    interpret_expr_list (world0 : world_state) (loc0 : string_map uint256) 
+                        (e : list expr)
+                        (CallOk0 : FSet.is_subset (expr_list_callset e)
+                                     (decl_callset (cached_const_folded_decl ok fc)) = true) {struct
+                        e} : world_state * Base.expr_result (list uint256) :=
+      match e as e' return (e = e' -> world_state * Base.expr_result (list uint256)) with
+      | nil => fun _ : e = nil => (world0, Base.ExprSuccess nil)
+      | (h :: t)%list =>
+          fun E : e = (h :: t)%list =>
+          let (world', result_h) :=
+            interpret_expr eq_refl (const_fold_fun_ctx ok fc) do_call' builtins world0 loc0 h
+              (callset_descend_head E CallOk0) in
+          match result_h with
+          | Base.ExprSuccess x =>
+              let (world'', result_t) :=
+                interpret_expr_list world' loc0 t (callset_descend_tail E CallOk0) in
+              (world'',
+              match result_t with
+              | Base.ExprSuccess y => Base.ExprSuccess (x :: y)%list
+              | Base.ExprAbort _ => result_t
+              end)
+          | Base.ExprAbort ab => (world', Base.ExprAbort ab)
+          end
+      end eq_refl) world loc args' Ok).
+  {
+    clear CallOk CallOk' Heqcargs ExprOk H1.
+    revert world loc. induction args'. { easy. }
+    intros. cbn.
+    assert (Irrel:
+        (@callset_descend_head C a args' (a :: args')
+          (@decl_callset C (@cached_const_folded_decl C (S smaller_call_depth_bound) cd cd' ok fc))
+          (@eq_refl (list (@expr C)) (a :: args')%list) Ok')
+         =
+        (@callset_descend_head C a args' (a :: args')
+          (@decl_callset C (@cached_const_folded_decl C (S smaller_call_depth_bound) cd cd' ok fc))
+          (@eq_refl (list (@expr C)) (a :: args')%list) Ok)).
+    { apply PropExtensionality.proof_irrelevance. }
+    rewrite Irrel.
+    destruct interpret_expr. destruct e. 2:{ trivial. }
+    now rewrite (IHargs' w loc 
+                  (@callset_descend_tail C a args' (a :: args')
+                    (@decl_callset C (@cached_const_folded_decl C (S smaller_call_depth_bound) cd cd' ok fc))
+                    (@eq_refl (list (@expr C)) (a :: args')%list) Ok')
+                  (@callset_descend_tail C a args' (a :: args')
+                    (@decl_callset C (@cached_const_folded_decl C (S smaller_call_depth_bound) cd cd' ok fc))
+                    (@eq_refl (list (@expr C)) (a :: args')%list) Ok)).
+  }
+  rewrite<- (R' (callset_descend_args eq_refl CallOk')). clear R'.
+  assert (W := weak_interpret_const_fold_expr_list builtins ok fc DoCallOk world loc Heqcargs
+                                                   (callset_descend_args eq_refl CallOk')
+                                                   (callset_descend_args eq_refl CallOk)
+                                                   H).
+  rewrite W.
+  assert (R:
+    forall Ok' Ok,
+    interpret_expr_list eq_refl fc do_call builtins world loc args Ok'
+     =
+    (fix
+      interpret_expr_list (world0 : world_state) (loc0 : string_map uint256) 
+                          (e : list expr)
+                          (CallOk0 : FSet.is_subset (expr_list_callset e) (decl_callset (fun_decl fc)) =
+                                     true) {struct e} : world_state * Base.expr_result (list uint256) :=
+        match e as e' return (e = e' -> world_state * Base.expr_result (list uint256)) with
+        | nil => fun _ : e = nil => (world0, Base.ExprSuccess nil)
+        | (h :: t)%list =>
+            fun E : e = (h :: t)%list =>
+            let (world', result_h) :=
+              interpret_expr eq_refl fc do_call builtins world0 loc0 h (callset_descend_head E CallOk0) in
+            match result_h with
+            | Base.ExprSuccess x =>
+                let (world'', result_t) :=
+                  interpret_expr_list world' loc0 t (callset_descend_tail E CallOk0) in
+                (world'',
+                match result_t with
+                | Base.ExprSuccess y => Base.ExprSuccess (x :: y)%list
+                | Base.ExprAbort _ => result_t
+                end)
+            | Base.ExprAbort ab => (world', Base.ExprAbort ab)
+            end
+        end eq_refl) world loc args Ok).
+  {
+    clear CallOk CallOk' Heqcargs args' W ExprOk H H1.
+    revert world loc. induction args. { easy. }
+    intros. cbn.
+    (* this is relatively horror-free this time: *)
+    assert (Irrel: callset_descend_head eq_refl Ok' = callset_descend_head eq_refl Ok).
+    { apply PropExtensionality.proof_irrelevance. }
+    rewrite Irrel.
+    destruct interpret_expr. destruct e. 2:{ trivial. }
+    now rewrite (IHargs w loc 
+                        (callset_descend_tail eq_refl Ok')
+                        (callset_descend_tail eq_refl Ok)).
+  }
+  rewrite<- (R (callset_descend_args eq_refl CallOk)). clear R.
+  remember (interpret_expr_list eq_refl fc do_call builtins world loc args
+             (callset_descend_args eq_refl CallOk)) as after_args. clear Heqafter_args.
+  destruct after_args as (world', result_args).
+  destruct result_args. 2:{ trivial. }
+  (* args computation has succeeded *)
+
+  enough (D: fun_ctx_descend (const_fold_fun_ctx ok fc)
+              CallOk' eq_refl eq_refl
+              =
+             match fun_ctx_descend fc CallOk eq_refl eq_refl with
+             | Some ctx => Some (const_fold_fun_ctx ok ctx)
+             | None => None
+             end).
+  {
+    rewrite D.
+    now destruct (fun_ctx_descend fc CallOk eq_refl eq_refl).
+  }
+  (* This follows the proof of D from From20To30/Expr.v, which in turn follows fun_ctx_descend_irrel. *)
+  unfold fun_ctx_descend.
+  assert (InnerOk: forall (d1 d2: decl)
+                          (Edecl1: cd_declmap cd  name = Some d1)
+                          (Edecl2: cd_declmap cd' name = Some d2),
+                 L20.Descend.fun_ctx_descend_inner (const_fold_fun_ctx ok fc) CallOk'
+                    eq_refl eq_refl Edecl2
+                  =
+                 match L20.Descend.fun_ctx_descend_inner fc CallOk eq_refl eq_refl Edecl1 with
+                 | Some ctx => Some (const_fold_fun_ctx ok ctx)
+                 | None => None
+                 end).
+  {
+    intros.
+    unfold Descend.fun_ctx_descend_inner.
+    remember (fun (depth: nat) (Edepth: cd_depthmap cd' name = Some depth) =>
+        Some
+          {|
+          fun_name := name;
+          fun_depth := depth;
+          fun_depth_ok := Edepth;
+          fun_decl := d2;
+          fun_decl_ok := Edecl2;
+          fun_bound_ok := Descend.call_descend' (const_fold_fun_ctx ok fc)
+                      CallOk' eq_refl eq_refl
+                            Edecl2 Edepth |})
+      as some_branch_l.
+    remember (fun Edepth : cd_depthmap cd' name = None =>
+                False_rect (option (fun_ctx cd' smaller_call_depth_bound))
+                           (Descend.fun_ctx_descend_helper Edecl2 Edepth))
+      as none_branch_l.
+    remember (fun (depth: nat) (Edepth: cd_depthmap cd name = Some depth) =>
+      Some
+        {|
+        fun_name := name;
+        fun_depth := depth;
+        fun_depth_ok := Edepth;
+        fun_decl := d1;
+        fun_decl_ok := Edecl1;
+        fun_bound_ok := Descend.call_descend' fc CallOk eq_refl eq_refl Edecl1 Edepth |})
+      as some_branch_r.
+    remember (fun Edepth : cd_depthmap cd name = None =>
+                  False_rect (option (fun_ctx cd smaller_call_depth_bound))
+                    (L20.Descend.fun_ctx_descend_helper Edecl1 Edepth))
+      as none_branch_r.
+    assert (NoneOkL: forall (Edepth: cd_depthmap cd' name = None),
+                       none_branch_l Edepth = None).
+    { intro. exfalso. exact (Descend.fun_ctx_descend_helper Edecl2 Edepth). }
+    assert (NoneOkR: forall (Edepth: cd_depthmap cd name = None),
+                       none_branch_r Edepth = None).
+    { intro. exfalso. exact (Descend.fun_ctx_descend_helper Edecl1 Edepth). }
+    clear Heqnone_branch_l Heqnone_branch_r.
+    revert none_branch_l none_branch_r NoneOkL NoneOkR.
+    assert (SomeBranchOk: forall (depth: nat)
+                                 (Edepth1: cd_depthmap cd name = Some depth)
+                                 (Edepth2: cd_depthmap cd' name = Some depth),
+                   some_branch_l depth Edepth2 
+                    =
+                   match some_branch_r depth Edepth1 with
+                   | Some ctx => Some (const_fold_fun_ctx ok ctx)
+                   | None => None
+                   end).
+    {
+      intros. subst. unfold const_fold_fun_ctx. cbn.
+      f_equal.
+      assert (D: d2 = cached_const_folded_decl ok
+              {|
+              fun_name := name;
+              fun_depth := depth;
+              fun_depth_ok := Edepth1;
+              fun_decl := d1;
+              fun_decl_ok := Edecl1;
+              fun_bound_ok := Descend.call_descend' fc CallOk eq_refl eq_refl Edecl1 Edepth1 |}).
+      {
+        unfold cached_const_folded_decl. cbn.
+        remember (translate_fun_ctx_fun_decl_helper ok _) as Bad. clear HeqBad.
+        cbn in Bad. revert Bad.
+        destruct (cd_declmap cd' name). { now inversion Edecl2. }
+        intro Bad. discriminate.
+      }
+      subst. f_equal; apply PropExtensionality.proof_irrelevance.
+    } (* SomeBranchOk *)
+    clear Heqsome_branch_l Heqsome_branch_r
+          CallOk CallOk' Edecl1 Edecl2 d1 d2 args value DoCallOk
+          do_call do_call' H Heqcargs W.
+    revert some_branch_l some_branch_r SomeBranchOk.
+    rewrite (const_fold_fun_ctx_depthmap ok name).
+    destruct (cd_depthmap cd' name), (cd_depthmap cd name); intros;
+      try apply SomeBranchOk; rewrite (NoneOkL eq_refl); rewrite (NoneOkR eq_refl); trivial.
+  } (* InnerOk *)
+  remember (@Descend.fun_ctx_descend_inner C (S smaller_call_depth_bound) smaller_call_depth_bound cd'
+             (@PrivateCall C name args') name args') as inner'.
+  remember (@Descend.fun_ctx_descend_inner C (S smaller_call_depth_bound) smaller_call_depth_bound cd
+             (@PrivateCall C name args) name args) as inner.
+  clear Heqinner' Heqinner.
+  subst.
+  remember (fun d (Edecl: cd_declmap cd' name = Some d) =>
+                inner' (const_fold_fun_ctx ok fc) CallOk' eq_refl eq_refl d Edecl)
+    as some_branch'.
+  remember (cd_declmap cd name) as maybe_d. destruct maybe_d.
+  {
+    assert (SomeBranchOk: forall (d': decl)
+                                 (Edecl: cd_declmap cd' name = Some d'),
+                   some_branch' d' Edecl
+                    =
+                   match inner fc CallOk eq_refl eq_refl d eq_refl with
+                   | Some ctx => Some (const_fold_fun_ctx ok ctx)
+                   | None => None
+                   end).
+    { intros. apply InnerOk. }
+    clear Heqsome_branch'.
+    remember (cd_declmap cd' name) as maybe_d'.
+    destruct maybe_d'. { apply SomeBranchOk. }
+    assert (T := const_fold_fun_ctx_declmap ok name).
+    rewrite<- Heqmaybe_d' in T.
+    rewrite<- Heqmaybe_d in T.
+    discriminate.
+  }
+  assert (SomeBranchOk: forall (d': decl)
+                               (Edecl: cd_declmap cd' name = Some d'),
+             some_branch' d' Edecl
+              =
+             None).
+  {
+    intros.
+    assert (T := const_fold_fun_ctx_declmap ok name).
+    rewrite<- Heqmaybe_d in T. rewrite Edecl in T.
+    discriminate.
+  }
+  clear Heqsome_branch'.
+  now destruct (cd_declmap cd' name).
+}
+(* BuiltinCall *)
+(* following PrivateCall until the args are computed successfully *)
+remember ((fix const_fold_expr_list (l : list expr) : string + list expr :=
+            match l with
+            | nil => inr nil
+            | (h :: t)%list =>
+                match const_fold_expr h with
+                | inl err => inl err
+                | inr h' =>
+                    match const_fold_expr_list t with
+                    | inl err => inl err
+                    | inr t' => inr (h' :: t')%list
+                    end
+                end
+            end) args) as cargs. symmetry in Heqcargs. destruct cargs. { discriminate. }
+inversion ExprOk. subst e'. cbn.
+rename l into args'.
+assert (R':
+  forall Ok' Ok,  (* initially: (callset_descend_args eq_refl CallOk') etc *)
+  interpret_expr_list eq_refl (const_fold_fun_ctx ok fc) do_call' builtins world loc args' Ok'
+   =
+  (fix
+  interpret_expr_list (world0 : world_state) (loc0 : string_map uint256) 
+                      (e : list expr)
+                      (CallOk0 : FSet.is_subset (expr_list_callset e)
+                                   (decl_callset (cached_const_folded_decl ok fc)) = true) {struct
+                      e} : world_state * Base.expr_result (list uint256) :=
+    match e as e' return (e = e' -> world_state * Base.expr_result (list uint256)) with
+    | nil => fun _ : e = nil => (world0, Base.ExprSuccess nil)
+    | (h :: t)%list =>
+        fun E : e = (h :: t)%list =>
+        let (world', result_h) :=
+          interpret_expr eq_refl (const_fold_fun_ctx ok fc) do_call' builtins world0 loc0 h
+            (callset_descend_head E CallOk0) in
+        match result_h with
+        | Base.ExprSuccess x =>
+            let (world'', result_t) :=
+              interpret_expr_list world' loc0 t (callset_descend_tail E CallOk0) in
+            (world'',
+            match result_t with
+            | Base.ExprSuccess y => Base.ExprSuccess (x :: y)%list
+            | Base.ExprAbort _ => result_t
+            end)
+        | Base.ExprAbort ab => (world', Base.ExprAbort ab)
+        end
+    end eq_refl) world loc args' Ok).
+{
+  clear CallOk CallOk' Heqcargs ExprOk H1.
+  revert world loc. induction args'. { easy. }
+  intros. cbn.
+  assert (Irrel:
+      (@callset_descend_head C a args' (a :: args')
+        (@decl_callset C (@cached_const_folded_decl C (S smaller_call_depth_bound) cd cd' ok fc))
+        (@eq_refl (list (@expr C)) (a :: args')%list) Ok')
+       =
+      (@callset_descend_head C a args' (a :: args')
+        (@decl_callset C (@cached_const_folded_decl C (S smaller_call_depth_bound) cd cd' ok fc))
+        (@eq_refl (list (@expr C)) (a :: args')%list) Ok)).
+  { apply PropExtensionality.proof_irrelevance. }
+  rewrite Irrel.
+  destruct interpret_expr. destruct e. 2:{ trivial. }
+  now rewrite (IHargs' w loc 
+                (@callset_descend_tail C a args' (a :: args')
+                  (@decl_callset C (@cached_const_folded_decl C (S smaller_call_depth_bound) cd cd' ok fc))
+                  (@eq_refl (list (@expr C)) (a :: args')%list) Ok')
+                (@callset_descend_tail C a args' (a :: args')
+                  (@decl_callset C (@cached_const_folded_decl C (S smaller_call_depth_bound) cd cd' ok fc))
+                  (@eq_refl (list (@expr C)) (a :: args')%list) Ok)).
+}
+rewrite<- (R' (callset_descend_builtin_args eq_refl CallOk')). clear R'.
+assert (W := weak_interpret_const_fold_expr_list builtins ok fc DoCallOk world loc Heqcargs
+                                                 (callset_descend_builtin_args eq_refl CallOk')
+                                                 (callset_descend_builtin_args eq_refl CallOk)
+                                                 H).
+rewrite W.
+assert (R:
+  forall Ok' Ok,
+  interpret_expr_list eq_refl fc do_call builtins world loc args Ok'
+   =
+  (fix
+    interpret_expr_list (world0 : world_state) (loc0 : string_map uint256) 
+                        (e : list expr)
+                        (CallOk0 : FSet.is_subset (expr_list_callset e) (decl_callset (fun_decl fc)) =
+                                   true) {struct e} : world_state * Base.expr_result (list uint256) :=
+      match e as e' return (e = e' -> world_state * Base.expr_result (list uint256)) with
+      | nil => fun _ : e = nil => (world0, Base.ExprSuccess nil)
+      | (h :: t)%list =>
+          fun E : e = (h :: t)%list =>
+          let (world', result_h) :=
+            interpret_expr eq_refl fc do_call builtins world0 loc0 h (callset_descend_head E CallOk0) in
+          match result_h with
+          | Base.ExprSuccess x =>
+              let (world'', result_t) :=
+                interpret_expr_list world' loc0 t (callset_descend_tail E CallOk0) in
+              (world'',
+              match result_t with
+              | Base.ExprSuccess y => Base.ExprSuccess (x :: y)%list
+              | Base.ExprAbort _ => result_t
+              end)
+          | Base.ExprAbort ab => (world', Base.ExprAbort ab)
+          end
+      end eq_refl) world loc args Ok).
+{
+  clear CallOk CallOk' Heqcargs args' W ExprOk H H1.
+  revert world loc. induction args. { easy. }
+  intros. cbn.
+  (* this is relatively horror-free this time: *)
+  assert (Irrel: callset_descend_head eq_refl Ok' = callset_descend_head eq_refl Ok).
+  { apply PropExtensionality.proof_irrelevance. }
+  rewrite Irrel.
+  destruct interpret_expr. destruct e. 2:{ trivial. }
+  now rewrite (IHargs w loc 
+                      (callset_descend_tail eq_refl Ok')
+                      (callset_descend_tail eq_refl Ok)).
+}
+rewrite<- (R (callset_descend_builtin_args eq_refl CallOk)). clear R.
+remember (interpret_expr_list eq_refl fc do_call builtins world loc args
+           (callset_descend_builtin_args eq_refl CallOk)) as after_args. clear Heqafter_args.
+destruct after_args as (world', result_args).
+now destruct result_args.
+Qed.
+
+
+Lemma interpret_const_fold_small_stmt {C: VyperConfig}
+                        {bigger_call_depth_bound smaller_call_depth_bound: nat}
+                        (Ebound: bigger_call_depth_bound = S smaller_call_depth_bound)
+                        (builtins: string -> option L10.Base.builtin)
+                        {cd cd': calldag}
+                        (ok: const_fold_calldag cd = inr cd')
+                        (fc: fun_ctx cd bigger_call_depth_bound)
+                        {do_call: forall
+                            (smaller_fc: fun_ctx cd smaller_call_depth_bound)
+                            (world: world_state)
+                            (arg_values: list uint256),
+                          world_state * L10.Base.expr_result uint256}
+                        {do_call': forall
+                              (smaller_fc: fun_ctx cd' smaller_call_depth_bound)
+                              (world: world_state)
+                              (arg_values: list uint256),
+                            world_state * L10.Base.expr_result uint256}
+                        (DoCallOk: forall smaller_fc world arg_values,
+                                     do_call' (const_fold_fun_ctx ok smaller_fc) world arg_values
+                                      =
+                                     do_call smaller_fc world arg_values)
+                        (world: world_state)
+                        (loc: string_map uint256)
+                        {ss ss': small_stmt}
+                        (StmtOk: const_fold_small_stmt ss = inr ss')
+                        (CallOk': let _ := string_set_impl in
+                           FSet.is_subset (small_stmt_callset ss')
+                                          (decl_callset
+                                             (fun_decl
+                                               (const_fold_fun_ctx ok fc)))
+                           = true)
+                        (CallOk: let _ := string_set_impl in
+                           FSet.is_subset (small_stmt_callset ss)
+                                          (decl_callset (fun_decl fc))
+                           = true):
+   interpret_small_stmt Ebound (const_fold_fun_ctx ok fc)
+                        do_call' builtins
+                        world loc ss' CallOk'
+    =
+   interpret_small_stmt Ebound fc
+                        do_call builtins
+                        world loc ss CallOk.
+Proof.
+destruct ss; cbn in StmtOk; unfold sum_map in *; cbn.
+{ (* Pass *) inversion StmtOk. now subst ss'. }
+{ (* Abort *) inversion StmtOk. now subst ss'. }
+{ (* Return *)
+  remember (const_fold_expr result) as result'. symmetry in Heqresult'.
+  destruct result'. { discriminate. }
+  inversion StmtOk. subst ss'.
+  cbn.
+  assert (R: @callset_descend_return C (@Return C e) e
+                (@decl_callset C (@cached_const_folded_decl C bigger_call_depth_bound cd cd' ok fc))
+                (@eq_refl (@small_stmt C) (@Return C e)) CallOk'
+              =
+             @callset_descend_return C (@Return C e) e
+                 (@decl_callset C (@fun_decl C (@decl C) (@decl_callset C) cd'
+                                bigger_call_depth_bound
+                               (@const_fold_fun_ctx C bigger_call_depth_bound cd cd' ok fc)))
+                 (@eq_refl (@small_stmt C) (@Return C e)) CallOk').
+  { easy. }
+  rewrite R.
+  rewrite (interpret_const_fold_expr Ebound builtins ok fc DoCallOk world loc Heqresult'
+                                          (callset_descend_return eq_refl CallOk')
+                                          (callset_descend_return eq_refl CallOk)).
+  now destruct interpret_expr.
+}
+{ (* Raise *) 
+  remember (const_fold_expr error) as error'. symmetry in Heqerror'.
+  destruct error'. { discriminate. }
+  inversion StmtOk. subst ss'.
+  cbn.
+  assert (R: @callset_descend_raise C (@Raise C e) e
+                (@decl_callset C (@cached_const_folded_decl C bigger_call_depth_bound cd cd' ok fc))
+                (@eq_refl (@small_stmt C) (@Raise C e)) CallOk'
+              =
+             @callset_descend_raise C (@Raise C e) e
+                 (@decl_callset C (@fun_decl C (@decl C) (@decl_callset C) cd'
+                                bigger_call_depth_bound
+                               (@const_fold_fun_ctx C bigger_call_depth_bound cd cd' ok fc)))
+                 (@eq_refl (@small_stmt C) (@Raise C e)) CallOk').
+  { easy. }
+  rewrite R.
+  rewrite (interpret_const_fold_expr Ebound builtins ok fc DoCallOk world loc Heqerror'
+                                          (callset_descend_raise eq_refl CallOk')
+                                          (callset_descend_raise eq_refl CallOk)).
+  now destruct interpret_expr.
+}
+{ (* Assign *)
+  remember (const_fold_expr rhs) as rhs'. symmetry in Heqrhs'.
+  destruct rhs'. { discriminate. }
+  inversion StmtOk. subst ss'.
+  cbn.
+  assert (R: @callset_descend_assign_rhs C (@Assign C lhs e) lhs e
+                (@decl_callset C (@cached_const_folded_decl C bigger_call_depth_bound cd cd' ok fc))
+                (@eq_refl (@small_stmt C) (@Assign C lhs e)) CallOk'
+              =
+             @callset_descend_assign_rhs C (@Assign C lhs e) lhs e
+                 (@decl_callset C (@fun_decl C (@decl C) (@decl_callset C) cd'
+                                bigger_call_depth_bound
+                               (@const_fold_fun_ctx C bigger_call_depth_bound cd cd' ok fc)))
+                 (@eq_refl (@small_stmt C) (@Assign C lhs e)) CallOk').
+  { easy. }
+  rewrite R.
+  rewrite (interpret_const_fold_expr Ebound builtins ok fc DoCallOk world loc Heqrhs'
+                                          (callset_descend_assign_rhs eq_refl CallOk')
+                                          (callset_descend_assign_rhs eq_refl CallOk)).
+  destruct interpret_expr as (world', result).
+  destruct result; cbn. 2:{ trivial. }
+  destruct lhs. { trivial. }
+  unfold storage_var_is_declared.
+  assert (D := const_fold_fun_ctx_declmap ok name).
+  destruct (cd_declmap cd' name), (cd_declmap cd name); try discriminate; trivial.
+  destruct d0; (* XXX *)
+    cbn in D; inversion D; subst; trivial.
+  unfold sum_map in *.
+  destruct (const_fold_stmt body). { discriminate. }
+  inversion D; subst. trivial.
+}
+(* ExprStmt *)
+remember (const_fold_expr e) as e'. symmetry in Heqe'.
+destruct e' as [|e']. { discriminate. }
+inversion StmtOk. subst ss'.
+cbn.
+rewrite<- (interpret_const_fold_expr Ebound builtins ok fc DoCallOk world loc Heqe'
+                                        (callset_descend_expr_stmt eq_refl CallOk')
+                                        (callset_descend_expr_stmt eq_refl CallOk)).
+
+assert (R: @callset_descend_expr_stmt C (@ExprStmt C e') e'
+            (@decl_callset C (@cached_const_folded_decl C bigger_call_depth_bound cd cd' ok fc))
+            (@eq_refl (@small_stmt C) (@ExprStmt C e')) CallOk'
+            =
+           @callset_descend_expr_stmt C (@ExprStmt C e') e'
+            (@decl_callset C
+               (@fun_decl C (@decl C) (@decl_callset C) cd' bigger_call_depth_bound
+                  (@const_fold_fun_ctx C bigger_call_depth_bound cd cd' ok fc)))
+            (@eq_refl (@small_stmt C) (@ExprStmt C e')) CallOk').
+{ easy. }
+rewrite R.
+now destruct interpret_expr.
+Qed.
+
+Lemma interpret_const_fold_stmt {C: VyperConfig}
+                        {bigger_call_depth_bound smaller_call_depth_bound: nat}
+                        (Ebound: bigger_call_depth_bound = S smaller_call_depth_bound)
+                        (builtins: string -> option L10.Base.builtin)
+                        {cd cd': calldag}
+                        (ok: const_fold_calldag cd = inr cd')
+                        (fc: fun_ctx cd bigger_call_depth_bound)
+                        {do_call: forall
+                            (smaller_fc: fun_ctx cd smaller_call_depth_bound)
+                            (world: world_state)
+                            (arg_values: list uint256),
+                          world_state * L10.Base.expr_result uint256}
+                        {do_call': forall
+                              (smaller_fc: fun_ctx cd' smaller_call_depth_bound)
+                              (world: world_state)
+                              (arg_values: list uint256),
+                            world_state * L10.Base.expr_result uint256}
+                        (DoCallOk: forall smaller_fc world arg_values,
+                                     do_call' (const_fold_fun_ctx ok smaller_fc) world arg_values
+                                      =
+                                     do_call smaller_fc world arg_values)
+                        (world: world_state)
+                        (loc: string_map uint256)
+                        {s s': stmt}
+                        (StmtOk: const_fold_stmt s = inr s')
+                        (CallOk': let _ := string_set_impl in
+                           FSet.is_subset (stmt_callset s')
+                                          (decl_callset
+                                             (fun_decl
+                                               (const_fold_fun_ctx ok fc)))
+                           = true)
+                        (CallOk: let _ := string_set_impl in
+                           FSet.is_subset (stmt_callset s)
+                                          (decl_callset (fun_decl fc))
+                           = true):
+   interpret_stmt Ebound (const_fold_fun_ctx ok fc)
+                  do_call' builtins
+                  world loc s' CallOk'
+    =
+   interpret_stmt Ebound fc
+                  do_call builtins
+                  world loc s CallOk.
+Proof.
+revert world loc s' StmtOk CallOk' CallOk.
+induction s; intros; cbn in StmtOk; unfold sum_map in *; unfold sum_ap in *.
+{ (* SmallStmt *)
+  remember (const_fold_small_stmt s) as ss'. symmetry in Heqss'.
+  destruct ss' as [|ss']. { discriminate. }
+  inversion StmtOk. subst s'. cbn.
+  now apply interpret_const_fold_small_stmt.
+}
+{ (* LocalVarDecl *)
+  remember (const_fold_expr init) as init'. symmetry in Heqinit'.
+  destruct init' as [|init']. { discriminate. }
+  destruct const_fold_stmt as [|body]. { discriminate. }
+  inversion StmtOk. subst s'. cbn.
+  destruct (Base.map_lookup loc name). { trivial. }
+  rewrite<- (interpret_const_fold_expr Ebound builtins ok fc DoCallOk world loc Heqinit'
+                                        (callset_descend_var_init eq_refl CallOk')
+                                        (callset_descend_var_init eq_refl CallOk)).
+  destruct interpret_expr as (world', result). destruct result. 2:{ trivial. }
+  assert (IH := IHs world' (Base.map_insert loc name value) body eq_refl
+                    (callset_descend_var_scope eq_refl CallOk')
+                    (callset_descend_var_scope eq_refl CallOk)).
+  assert (R: (@callset_descend_var_scope C (@LocalVarDecl C name init' body) name init' body
+               (@decl_callset C (@cached_const_folded_decl C bigger_call_depth_bound cd cd' ok fc))
+               (@eq_refl (@stmt C) (@LocalVarDecl C name init' body)) CallOk')
+              =
+             (@callset_descend_var_scope C (@LocalVarDecl C name init' body) name init' body
+               (@decl_callset C
+                 (@fun_decl C (@decl C) (@decl_callset C) cd' bigger_call_depth_bound
+                 (@const_fold_fun_ctx C bigger_call_depth_bound cd cd' ok fc)))
+               (@eq_refl (@stmt C) (@LocalVarDecl C name init' body)) CallOk')).
+  { easy. }
+  rewrite R.
+  now rewrite IH.
+}
+{ (* IfElseStmt *)
+  rename s1 into yes. rename s2 into no. rename IHs1 into IHyes. rename IHs2 into IHno.
+  remember (const_fold_expr cond) as cond'. symmetry in Heqcond'.
+  destruct cond' as [|cond']. { discriminate. }
+  remember (const_fold_stmt yes) as yes'. symmetry in Heqyes'.
+  destruct yes' as [|yes']. { discriminate. }
+  remember (const_fold_stmt no) as no'. symmetry in Heqno'.
+  destruct no' as [|no']. { discriminate. }
+  inversion StmtOk. subst s'. cbn.
+  rewrite<- (interpret_const_fold_expr Ebound builtins ok fc DoCallOk world loc Heqcond'
+                   (callset_descend_stmt_if_cond eq_refl CallOk')
+                   (callset_descend_stmt_if_cond eq_refl CallOk)).
+  destruct interpret_expr as (world', result). destruct result. 2:{ trivial. }
+  destruct (Z_of_uint256 value =? 0)%Z.
+  { (* no *)
+    apply (IHno _ _ _ eq_refl (callset_descend_stmt_if_else eq_refl CallOk')
+                              (callset_descend_stmt_if_else eq_refl CallOk)).
+  }
+  apply (IHyes _ _ _ eq_refl (callset_descend_stmt_if_then eq_refl CallOk')
+                             (callset_descend_stmt_if_then eq_refl CallOk)).
+}
+2:{ (* Semicolon *)
+  remember (const_fold_stmt s1) as s1'. symmetry in Heqs1'.
+  destruct s1' as [|s1']. { discriminate. }
+  remember (const_fold_stmt s2) as s2'. symmetry in Heqs2'.
+  destruct s2' as [|s2']. { discriminate. }
+  inversion StmtOk. subst s'. cbn.
+  rewrite (IHs1 _ _ _ eq_refl (callset_descend_semicolon_left eq_refl CallOk')
+                              (callset_descend_semicolon_left eq_refl CallOk)).
+  destruct interpret_stmt as ((world', loc'), result). destruct result; trivial.
+  apply (IHs2 _ _ _ eq_refl (callset_descend_semicolon_right eq_refl CallOk')
+                            (callset_descend_semicolon_right eq_refl CallOk)).
+}
+(* Loop *)
+remember (const_fold_expr start) as start'. symmetry in Heqstart'.
+destruct start' as [|start']. { discriminate. }
+rename s into body. remember (const_fold_stmt body) as body'. symmetry in Heqbody'.
+destruct body' as [|body']. { discriminate. }
+inversion StmtOk. subst s'. cbn.
+remember (Base.map_lookup loc var) as lookup_var.
+destruct lookup_var. { trivial. }
+remember (Z_of_uint256 count =? 0)%Z as count_is_0.
+destruct count_is_0. { trivial. }
+rewrite<- (interpret_const_fold_expr Ebound builtins ok fc DoCallOk world loc Heqstart'
+                   (callset_descend_loop_start eq_refl CallOk')
+                   (callset_descend_loop_start eq_refl CallOk)).
+destruct interpret_expr as (world', result_start).
+destruct result_start. 2:{ trivial. }
+remember (Z_of_uint256 (uint256_of_Z (Z_of_uint256 value + Z_of_uint256 count - 1)) =?
+           Z_of_uint256 value + Z_of_uint256 count - 1)%Z
+  as no_overflow.
+destruct no_overflow. 2:{ trivial. }
+(* checks completed, now the loop itself *)
+remember (Z.to_nat (Z_of_uint256 count)) as countdown.
+remember (Z_of_uint256 value) as cursor.
+
+(* closely following From20To30/Stmt.v here *)
+remember (Z_of_uint256 value + Z_of_uint256 count - 1)%Z as cap.
+assert (CapRange: (0 <= cap < 2 ^ 256)%Z).
+{
+  symmetry in Heqno_overflow. rewrite Z.eqb_eq in Heqno_overflow.
+  rewrite uint256_ok in Heqno_overflow.
+  rewrite Z.mod_small_iff in Heqno_overflow by apply two_to_256_ne_0.
+  subst cursor cap.
+  enough (~ (2 ^ 256 < (Z_of_uint256 value + Z_of_uint256 count - 1)%Z <= 0)%Z). 
+  { tauto. }
+  intro Y.
+  assert (Bad := proj2 (Z.ltb_lt _ _) (Z.lt_le_trans _ _ _ (proj1 Y) (proj2 Y))).
+  cbn in Bad. discriminate.
+}
+
+assert (WeakMainLoopEq: 
+          cap = (cursor + Z_of_uint256 count - 1)%Z
+           \/
+          Z_of_uint256 count = 0%Z).
+{ left. subst cursor. exact Heqcap. }
+
+clear Heqcap Heqcursor world Heqno_overflow Heqcount_is_0 Heqlookup_var.
+revert count world' loc cursor WeakMainLoopEq CallOk' CallOk Heqcountdown StmtOk.
+induction countdown; intros. { trivial. } (* ----------- induction -------------*)
+rewrite (IHs _ _ _ eq_refl (callset_descend_loop_body eq_refl CallOk')
+                           (callset_descend_loop_body eq_refl CallOk)).
+
+(* checking that the counter doesn't go below 0 *)
+pose (count' := uint256_of_Z (Z.pred (Z_of_uint256 count))).
+assert (CountOk: countdown = Z.to_nat (Z_of_uint256 count')).
+{
+  unfold count'. rewrite uint256_ok.
+  assert (R := uint256_range count).
+  remember (Z_of_uint256 count) as z. clear Heqz.
+  assert (W: z = Z.succ (Z.of_nat countdown)).
+  {
+    rewrite<- Nat2Z.inj_succ. rewrite Heqcountdown.
+    symmetry. apply Z2Nat.id. tauto.
+  }
+  subst z. rewrite Z.pred_succ.
+  replace (Z.of_nat countdown mod 2 ^ 256)%Z with (Z.of_nat countdown).
+  { symmetry. apply Nat2Z.id. }
+  symmetry. apply Z.mod_small.
+  split.
+  { (* 0 <= countdown *) apply Nat2Z.is_nonneg. }
+  exact (Z.lt_trans _ _ _ (Z.lt_succ_diag_r (Z.of_nat countdown)) (proj2 R)).
+}
+
+(* strengthening WeakMainLoopEq *)
+assert (MainLoopEq: cap = (cursor + Z_of_uint256 count - 1)%Z).
+{
+  enough (Z_of_uint256 count <> 0%Z). { tauto. }
+  intro J. rewrite J in *.
+  cbn in Heqcountdown. discriminate.
+}
+
+assert (NextLoopEq: cap = (Z.succ cursor + Z_of_uint256 count' - 1)%Z).
+{
+  rewrite MainLoopEq.
+  enough (Z_of_uint256 count = Z_of_uint256 count' + 1)%Z by lia.
+  subst countdown.
+  assert (R := uint256_range count).
+  assert (R' := uint256_range count').
+  lia.
+}
+
+assert (WeakNextLoopEq: (cap = Z.succ cursor + Z_of_uint256 count' - 1 \/ Z_of_uint256 count' = 0)%Z).
+{ left. apply NextLoopEq. }
+
+destruct (interpret_stmt Ebound fc do_call builtins world'
+            (Base.map_insert loc var (uint256_of_Z cursor))
+            body (callset_descend_loop_body eq_refl CallOk)) as ((world''', loc'''), result''').
+
+assert (IH := IHcountdown count' world''' loc''' (Z.succ cursor)
+                          WeakNextLoopEq CallOk' CallOk CountOk eq_refl).
+assert (FixCallL:
+ (@callset_descend_loop_body C (@Loop C var start' count' body') body' var start' count'
+                (@decl_callset C (@cached_const_folded_decl C bigger_call_depth_bound cd cd' ok fc))
+                (@eq_refl (@stmt C) (@Loop C var start' count' body')) CallOk')
+  =
+ (@callset_descend_loop_body C (@Loop C var start' count body') body' var start' count
+               (@decl_callset C (@cached_const_folded_decl C bigger_call_depth_bound cd cd' ok fc))
+               (@eq_refl (@stmt C) (@Loop C var start' count body')) CallOk'))
+  by apply PropExtensionality.proof_irrelevance.
+assert (FixCallR:
+   (@callset_descend_loop_body C (@Loop C var start count' body) body var start count'
+    (@decl_callset C
+       (@fun_decl C (@decl C) (@decl_callset C) cd bigger_call_depth_bound fc))
+    (@eq_refl (@stmt C) (@Loop C var start count' body)) CallOk)
+  =
+ (@callset_descend_loop_body C (@Loop C var start count body) body var start count
+   (@decl_callset C
+      (@fun_decl C (@decl C) (@decl_callset C) cd bigger_call_depth_bound fc))
+   (@eq_refl (@stmt C) (@Loop C var start count body)) CallOk))
+  by apply PropExtensionality.proof_irrelevance.
+rewrite FixCallL in IH. rewrite FixCallR in IH. clear FixCallL FixCallR.
+destruct result'''; try trivial.
+now destruct a.
+Qed.
+
+(* XXX XXX XXX shit happens if this is placed in the beginning *)
+From Vyper.L20 Require Import Interpret.
+
+Lemma interpret_const_fold_call {C: VyperConfig}
+                                (builtins: string -> option L10.Base.builtin)
+                                {cd cd': calldag}
+                                (ok: const_fold_calldag cd = inr cd')
+                                {call_depth_bound: nat}
+                                (fc: fun_ctx cd call_depth_bound)
+                                (world: world_state)
+                                (arg_values: list uint256):
+  interpret_call builtins (const_fold_fun_ctx ok fc) world arg_values
+   =
+  interpret_call builtins fc world arg_values.
+Proof.
+revert world arg_values. induction call_depth_bound.
+{ exfalso. exact (Nat.nlt_0_r _ (proj1 (Nat.ltb_lt _ _) (fun_bound_ok fc))). }
+assert(F: inr (cached_const_folded_decl ok fc)
+           =
+          const_fold_decl (fun_decl fc)).
+{
+  clear IHcall_depth_bound.
+  unfold const_fold_fun_ctx in *. cbn in *.
+  unfold cached_const_folded_decl in *.
+  remember (translate_fun_ctx_fun_decl_helper ok fc) as foo. clear Heqfoo.
+  remember (cd_declmap cd' (fun_name fc)) as d.
+  destruct d. 2:{ contradiction. }
+  subst.
+  assert (Q := const_fold_fun_ctx_declmap ok (fun_name fc)).
+  destruct (cd_declmap cd' (fun_name fc)) as [d'|]. 2:discriminate.
+  inversion Heqd. subst d'. clear Heqd.
+  remember (cd_declmap cd (fun_name fc)) as x.
+  destruct x as [x|]. 2:discriminate.
+  inversion Q. f_equal.
+  assert (D := fun_decl_ok fc).
+  rewrite D in *. inversion Heqx.
+  trivial.
+}
+intros.
+cbn.
+remember (fun name arg_names body
+              (E : cached_const_folded_decl ok fc = FunDecl name arg_names body) =>
+    match Interpret.bind_args arg_names arg_values with
+    | inl err => (world, Base.expr_error err)
+    | inr loc =>
+        let
+        '(world', _, result) :=
+         interpret_stmt eq_refl (const_fold_fun_ctx ok fc) (interpret_call builtins) builtins world
+           loc body (Interpret.interpret_call_helper E) in
+         (world',
+         match result with
+         | Base.StmtSuccess => Base.ExprSuccess zero256
+         | Base.StmtAbort a => Base.ExprAbort a
+         | Base.StmtReturnFromFunction x => Base.ExprSuccess x
+         end)
+    end) as branch_l.
+remember (fun name arg_names body
+              (E : fun_decl fc = FunDecl name arg_names body) =>
+          match Interpret.bind_args arg_names arg_values with
+          | inl err => (world, Base.expr_error err)
+          | inr loc =>
+              let
+              '(world', _, result) :=
+               interpret_stmt eq_refl fc (interpret_call builtins) builtins world loc body
+                 (Interpret.interpret_call_helper E) in
+               (world',
+               match result with
+               | Base.StmtSuccess => Base.ExprSuccess zero256
+               | Base.StmtAbort a => Base.ExprAbort a
+               | Base.StmtReturnFromFunction x => Base.ExprSuccess x
+               end)
+          end) as branch_r.
+enough (B: forall name arg_names body_l body_r E_l E_r,
+             branch_l name arg_names body_l E_l
+              =
+             branch_r name arg_names body_r E_r).
+{
+  clear Heqbranch_l Heqbranch_r.
+  destruct (fun_decl fc); cbn in F; destruct cached_const_folded_decl;
+    unfold sum_map in *; try destruct (const_fold_stmt body); try easy.
+  inversion F; subst.
+  apply B.
+}
+intros. subst.
+rewrite E_l in F. rewrite E_r in F. cbn in F.
+destruct (Interpret.bind_args arg_names arg_values) as [|loc]. { trivial. }
+enough (E: interpret_stmt eq_refl (const_fold_fun_ctx ok fc) (interpret_call builtins) builtins world loc
+                          body_l (Interpret.interpret_call_helper E_l)
+            =
+           interpret_stmt eq_refl fc (interpret_call builtins) builtins world loc body_r
+                          (Interpret.interpret_call_helper E_r)).
+{ rewrite E. now destruct interpret_stmt. }
+apply interpret_const_fold_stmt.
+{ apply IHcall_depth_bound. }
+unfold sum_map in F. destruct (const_fold_stmt body_r). { discriminate. }
+inversion F. now subst.
+Qed.
